

COMP 4900D: Assignment 1 Solutions

1. (a) $\cos(\phi_1 + \phi_2) = \cos\phi_1 \cos\phi_2 - \sin\phi_1 \sin\phi_2$, $\sin(\phi_1 + \phi_2) = \sin\phi_1 \cos\phi_2 + \cos\phi_1 \sin\phi_2$

$$R(\phi_1 + \phi_2) = \begin{bmatrix} \cos(\phi_1 + \phi_2) & \sin(\phi_1 + \phi_2) \\ -\sin(\phi_1 + \phi_2) & \cos(\phi_1 + \phi_2) \end{bmatrix} = \begin{bmatrix} \cos\phi_1 \cos\phi_2 - \sin\phi_1 \sin\phi_2 & \sin\phi_1 \cos\phi_2 + \cos\phi_1 \sin\phi_2 \\ -\sin\phi_1 \cos\phi_2 - \cos\phi_1 \sin\phi_2 & \cos\phi_1 \cos\phi_2 - \sin\phi_1 \sin\phi_2 \end{bmatrix}$$

$$R(\phi_1)R(\phi_2) = \begin{bmatrix} \cos\phi_1 & \sin\phi_1 \\ -\sin\phi_1 & \cos\phi_1 \end{bmatrix} \begin{bmatrix} \cos\phi_2 & \sin\phi_2 \\ -\sin\phi_2 & \cos\phi_2 \end{bmatrix} = \begin{bmatrix} \cos\phi_1 \cos\phi_2 - \sin\phi_1 \sin\phi_2 & \cos\phi_1 \sin\phi_2 + \sin\phi_1 \cos\phi_2 \\ -\sin\phi_1 \cos\phi_2 - \cos\phi_1 \sin\phi_2 & \cos\phi_1 \cos\phi_2 - \sin\phi_1 \sin\phi_2 \end{bmatrix}$$

(b) $R(\phi)R(-\phi) = \begin{bmatrix} \cos\phi & \sin\phi \\ -\sin\phi & \cos\phi \end{bmatrix} \begin{bmatrix} \cos\phi & -\sin\phi \\ \sin\phi & \cos\phi \end{bmatrix} = \begin{bmatrix} 1 & 0 \\ 0 & 1 \end{bmatrix}$

2. (a) $x' = sx$ $y' = sy$ $\begin{bmatrix} x' \\ y' \end{bmatrix} = \begin{bmatrix} s & 0 \\ 0 & s \end{bmatrix} \begin{bmatrix} x \\ y \end{bmatrix}$

(b) $\begin{bmatrix} x' \\ y' \\ 1 \end{bmatrix} = \begin{bmatrix} s & 0 & 0 \\ 0 & s & 0 \\ 0 & 0 & 1 \end{bmatrix} \begin{bmatrix} x \\ y \\ 1 \end{bmatrix}$

(c) $\begin{bmatrix} x' \\ y' \\ 1 \end{bmatrix} = \begin{bmatrix} s & 0 & t_x \\ 0 & s & t_y \\ 0 & 0 & 1 \end{bmatrix} \begin{bmatrix} x \\ y \\ 1 \end{bmatrix}$

(d) $\begin{bmatrix} x' \\ y' \\ z' \\ 1 \end{bmatrix} = \begin{bmatrix} s & 0 & 0 & t_x \\ 0 & s & 0 & t_y \\ 0 & 0 & s & t_z \\ 0 & 0 & 0 & 1 \end{bmatrix} \begin{bmatrix} x \\ y \\ z \\ 1 \end{bmatrix}$

3. normal equation $ATAx = A^Tb$

$$\begin{bmatrix} 1 & 0 & 1 \\ 0 & 1 & 1 \end{bmatrix} \begin{bmatrix} 1 & 0 \\ 0 & 1 \\ 1 & 1 \end{bmatrix} \begin{bmatrix} x_1 \\ x_2 \end{bmatrix} = \begin{bmatrix} 1 & 0 & 1 \\ 0 & 1 & 1 \end{bmatrix} \begin{bmatrix} 1 \\ 0 \end{bmatrix}$$

$$\begin{bmatrix} 2 & 1 \\ 1 & 2 \end{bmatrix} \begin{bmatrix} x_1 \\ x_2 \end{bmatrix} = \begin{bmatrix} 1 \\ 1 \end{bmatrix} \quad \bar{x} = \begin{bmatrix} x_1 \\ x_2 \end{bmatrix} = \begin{bmatrix} 1/3 \\ 1/3 \end{bmatrix}$$

4. (a) $P = \begin{bmatrix} -500 & 0 & 320 \\ 0 & -500 & 240 \\ 0 & 0 & 1 \end{bmatrix} \begin{bmatrix} 0 & 1 & 0 & 70 \\ -1 & 0 & 0 & 95 \\ 0 & 0 & 1 & 120 \end{bmatrix} = \begin{bmatrix} 0 & -500 & 320 & 3400 \\ 500 & 0 & 240 & -18700 \\ 0 & 0 & 1 & 120 \end{bmatrix}$

(b) $X_h = P \begin{bmatrix} 150 \\ 200 \\ 400 \\ 1 \end{bmatrix} = \begin{bmatrix} 31400 \\ 152300 \\ 520 \end{bmatrix}$

$$X_{im} = \begin{bmatrix} X_h[1]/X_h[3] \\ X_h[2]/X_h[3] \end{bmatrix} = \begin{bmatrix} 60.38 \\ 292.88 \end{bmatrix}$$